

Problem 1

X_1, \dots, X_n are independent and $X_i \sim \text{Poisson}(2)$, $i = 1, \dots, n$

$$\begin{aligned} P(\min(X_1, \dots, X_n) > m) &= P(X_1 > m) \cdots P(X_n > m) = \prod_{i=1}^n P(X_i > m) \\ &= P(X_1 > m)^n = [1 - P(X_1 \leq m)]^n \end{aligned}$$

Since $P(X_i = k) = \frac{e^{-2} 2^k}{k!}$, $P(X_1 \leq m) = e^{-2} \sum_{i=0}^m \frac{2^i}{i!}$

$$P(\min(X_1, \dots, X_n) > m) = \left[1 - e^{-2} \sum_{i=0}^m \frac{2^i}{i!} \right]^n$$

$$\begin{aligned} P(\max(X_1, \dots, X_n) \leq m) &= P(X_1 \leq m) \cdots P(X_n \leq m) = P(X_1 \leq m)^n \\ &= \left(e^{-2} \sum_{i=0}^m \frac{2^i}{i!} \right)^n \end{aligned}$$

Problem 2

$$(a) \quad P_{XY}(x, y) = \begin{cases} \frac{(1-p)p^{x-1}x^y e^{-x}}{y!}, & x \geq 1, y \geq 0 \\ 0, & \text{otherwise} \end{cases}$$

$$\begin{aligned} P_X(x) &= \sum_{y=0}^{\infty} P_{XY}(x, y) = \sum_{y=0}^{\infty} \frac{(1-p)p^{x-1}x^y e^{-x}}{y!} = (1-p)p^{x-1}e^{-x} \sum_{y=0}^{\infty} \frac{x^y}{y!} \\ &= (1-p)p^{x-1}e^{-x} \cdot e^x = (1-p)p^{x-1} \end{aligned}$$

Therefore, $P_X(x) = \begin{cases} (1-p)p^{x-1}, & x \geq 1 \\ 0, & \text{otherwise} \end{cases}$

$$(b) \quad P_Y(y) = \sum_{x=1}^{\infty} P_{XY}(x, y) = \sum_{x=1}^{\infty} \frac{(1-p)p^{x-1}x^y e^{-x}}{y!}, \quad y \geq 0$$

$$\begin{aligned} P_Y(0) &= \sum_{x=1}^{\infty} \frac{(1-p)p^{x-1} \cdot 1 \cdot e^{-x}}{1} = \frac{1-p}{p} \sum_{x=1}^{\infty} p^x \cdot e^{-x} = \frac{1-p}{p} \sum_{x=1}^{\infty} (pe^{-1})^x \\ &= \frac{1-p}{p} \left(\frac{1}{1-pe^{-1}} - 1 \right) = \frac{1-p}{p} \cdot \frac{pe^{-1}}{1-pe^{-1}} = \frac{(1-p)e^{-1}}{1-pe^{-1}} \end{aligned}$$

$$\begin{aligned} (c) \quad P_X(x) P_Y(y) &= (1-p)p^{x-1} \cdot \frac{1-p}{y!} \sum_{x=1}^{\infty} p^{x-1} x^y e^{-x} \\ &= \frac{(1-p)^2 p^{x-1}}{y!} \sum_{x=1}^{\infty} p^{x-1} x^y e^{-x}, \quad x \geq 1, y \geq 0 \end{aligned}$$

$$\neq P_{XY}(x, y)$$

Thus, X and Y are not independent.

Problem 3

$$(a) f(x) = \begin{cases} \lambda p x^{p-1} e^{-\lambda x^p}, & x > 0 \\ 0, & x \leq 0 \end{cases}, \text{ where } \lambda > 0 \text{ and } p > 0$$

$$\int_{-\infty}^{+\infty} f(x) dx = \int_0^{+\infty} f(x) dx = \int_0^{+\infty} \lambda p x^{p-1} e^{-\lambda x^p} dx$$

$$\text{let } u = \lambda x^p, \frac{du}{dx} = \lambda p x^{p-1}, du = \lambda p x^{p-1} dx$$

$$\int_0^{+\infty} \lambda p x^{p-1} e^{-\lambda x^p} dx = \int_0^{+\infty} e^{-u} du = -e^{-u} \Big|_{u=+\infty} - (-e^{-u}) \Big|_{u=0} = 1$$

Thus, this density integrates to 1

$$\begin{aligned} (b) P(\text{at least one } X_i > 3) &= 1 - P(\text{none of } X_i > 3) \\ &= 1 - P(\text{all } X_i \leq 3) = 1 - P(X_1 \leq 3) \cdots P(X_n \leq 3) \\ &= 1 - P(X_1 \leq 3)^n \end{aligned}$$

$$\text{since } u = \lambda x^p, u(0) = 0, u(3) = \lambda 3^p$$

$$\begin{aligned} P(X_1 \leq 3) &= \int_0^3 \lambda p x^{p-1} e^{-\lambda x^p} dx = \int_0^{\lambda 3^p} e^{-u} du = -e^{-u} \Big|_{u=\lambda 3^p} - (-e^{-u}) \Big|_{u=0} \\ &= 1 - e^{-\lambda 3^p} \end{aligned}$$

$$P(\text{at least one } X_i > 3) = 1 - P(X_1 \leq 3)^n = 1 - (1 - e^{-\lambda 3^p})^n$$

Problem 4

A probability density function f must satisfy $f(x) \geq 0$ for all x and $\int_{-\infty}^{+\infty} f(x) dx = 1$

$$\text{Since } f(z) = \frac{1}{B(p, q)} \cdot \frac{z^{p-1}}{(1+z)^{p+q}}, z > 0, B(p, q) = \int_0^1 u^{p-1} (1-u)^{q-1} du, p > 0, q > 0$$

$$u \in (0, 1), u^{p-1} > 0, (1-u)^{q-1} > 0, B(p, q) > 0, z^{p-1} > 0, (1+z)^{p+q} > 0$$

$\Rightarrow f(z) \geq 0$ for all z

$$\int_{-\infty}^{+\infty} f(z) dz = \int_0^{+\infty} f(z) dz = \frac{1}{B(p, q)} \int_0^{+\infty} \frac{z^{p-1}}{(1+z)^{p+q}} dz$$

$$\text{let } t = \frac{1}{1+z}, \quad z = \frac{1-t}{t}, \quad \frac{dz}{dt} = -\frac{1}{t^2}, \quad dz = -\frac{1}{t^2} dt$$

when $z=0$, $t=1$, when $z=+\infty$, $t=0$

$$\begin{aligned} \int_0^{+\infty} \frac{z^{p-1}}{(1+z)^{p+q}} dz &= \int_1^0 \frac{\left(\frac{1-t}{t}\right)^{p-1}}{\left(1+\frac{1-t}{t}\right)^{p+q}} \left(-\frac{1}{t^2}\right) dt \\ &= \int_0^1 t^{p+q} \frac{(1-t)^{p-1}}{t^{p-1}} \frac{1}{t^2} dt = \int_0^1 t^{q-1} (1-t)^{p-1} dt \end{aligned}$$

$$\text{let } v = 1-t, \quad t = 1-v \quad \frac{dt}{dv} = -1, \quad dt = -dv$$

when $t=0$, $v=1$, when $t=1$, $v=0$

$$\int_0^1 t^{q-1} (1-t)^{p-1} dt = \int_1^0 (1-v)^{q-1} v^{p-1} (-1) dv = \int_0^1 v^{p-1} (1-v)^{q-1} dv = B(p, q)$$

$$\text{Thus, } \int_{-\infty}^{+\infty} f(z) dz = \frac{1}{B(p, q)} \int_0^{+\infty} \frac{z^{p-1}}{(1+z)^{p+q}} dz = \frac{B(p, q)}{B(p, q)} = 1$$

Therefore, $f(z)$ is a valid density

Problem 5

Since $f_n(x)$ is a probability density function, $f_n(x) \geq 0$ for all x ,

Since, $p_n \geq 0$ for all n , $f(x) = \sum_n p_n f_n(x) \geq 0$ for all x

$$\int_{-\infty}^{+\infty} f(x) dx = \int_{-\infty}^{+\infty} \sum_n p_n f_n(x) dx = \sum_n p_n \int_{-\infty}^{+\infty} f_n(x) dx = \sum_n p_n = 1$$

Therefore, $f(x) = \sum_n p_n f_n(x)$ is a probability density function

Problem 6

Since $X \sim \text{Weibull}(p, \lambda)$, then $f(x) = \begin{cases} \lambda p x^{p-1} e^{-\lambda x^p}, & x > 0 \\ 0, & x \leq 0 \end{cases}$

$$E(X^n) = \int_{-\infty}^{+\infty} x^n f(x) dx = \int_0^{+\infty} x^n \lambda p x^{p-1} e^{-\lambda x^p} dx$$

$$\text{let } u = \lambda x^p, \quad \frac{du}{dx} = \lambda p x^{p-1}, \quad du = \lambda p x^{p-1} dx, \quad x = \left(\frac{u}{\lambda}\right)^{\frac{1}{p}}$$

$$E(X^n) = \int_0^{+\infty} x^n e^{-u} du = \int_0^{+\infty} \left(\frac{u}{\lambda}\right)^{\frac{n}{p}} e^{-u} du$$

$$\text{Since } \Gamma(z) = \int_0^{+\infty} t^{z-1} e^{-t} dt, \quad \Gamma\left(1 + \frac{n}{p}\right) = \int_0^{+\infty} t^{\frac{n}{p}} e^{-t} dt$$

$$\text{Thus, } E(X^n) = \frac{\Gamma(1 + \frac{n}{p})}{\lambda^{n/p}}$$

Problem 7

$$X \sim \text{Exp}(1), \quad f_X(x) = \begin{cases} e^{-x}, & x \geq 0 \\ 0, & x < 0 \end{cases}, \quad F_X(x) = \begin{cases} 1 - e^{-x}, & x \geq 0 \\ 0, & x < 0 \end{cases}$$

We want to show that $Y = \sqrt{X} \sim \text{Rayleigh}(\frac{1}{\sqrt{2}})$, $f_Y(y) = 2ye^{-y^2}$, $y \geq 0$

$$\begin{aligned} \text{So, we have } F_Y(y) &= P(Y \leq y) = P(\sqrt{X} \leq y) = P(X \leq y^2) \\ &= F_X(y^2) = 1 - e^{-y^2}, \quad y \geq 0 \end{aligned}$$

$$f_Y(y) = \frac{dF_Y(y)}{dy} = 2ye^{-y^2}, \quad y \geq 0$$

Therefore, $Y = \sqrt{X} \sim \text{Rayleigh}(\frac{1}{\sqrt{2}})$

Problem 8

$X, Y \sim \text{Exp}(\lambda)$, X and Y are independent, $F_X(x) = 1 - e^{-\lambda x}$, $F_Y(y) = 1 - e^{-\lambda y}$
 $x \in [0, +\infty)$

let $U = \max(X, Y)$

$$\text{Thus, } F_U(u) = P(U \leq u) = P(\max(X, Y) \leq u) = P(X \leq u \text{ and } Y \leq u)$$

$$= P(X \leq u) \cdot P(Y \leq u) = (1 - e^{-\lambda u})^2$$

$$\begin{aligned} f_U(u) &= \frac{dF_U(u)}{du} = \frac{dF_U(u)}{dv} \cdot \frac{dv}{du} = 2(1 - e^{-\lambda u}) \lambda e^{-\lambda u} \\ (v = 1 - e^{-\lambda u}) &= 2\lambda e^{-\lambda u}(1 - e^{-\lambda u}) \end{aligned}$$

$$E(U) = \int_{-\infty}^{+\infty} u f_U(u) du = \int_0^{+\infty} 2u \lambda e^{-\lambda u} (1 - e^{-\lambda u}) du$$

$$= 2 \int_0^{+\infty} \lambda u e^{-\lambda u} - \lambda u e^{-2\lambda u} du$$

$$= 2 \int_0^{+\infty} \lambda u e^{-\lambda u} du - 2 \int_0^{+\infty} \lambda u e^{-2\lambda u} du$$

$$\text{let } v = \lambda u, \quad \frac{dv}{du} = \lambda, \quad dv = \lambda du$$

$$E(U) = 2 \int_0^{+\infty} \frac{v}{\lambda} e^{-v} dv - 2 \int_0^{+\infty} \frac{v}{\lambda} e^{-2v} dv$$

$$\begin{aligned}
&= \frac{2}{\lambda} \int_0^{+\infty} v e^{-v} dv - \frac{2}{\lambda} \int_0^{+\infty} v e^{-2v} dv \\
&= \frac{2}{\lambda} \left(- \int_0^{+\infty} v d(e^{-v}) \right) - \frac{2}{\lambda} \left(\frac{1}{2} \int_0^{+\infty} v d(e^{-2v}) \right) \\
&= -\frac{2}{\lambda} \left(v e^{-v} \Big|_0^{+\infty} - \int_0^{+\infty} e^{-v} dv \right) + \frac{1}{\lambda} \left(v e^{-2v} \Big|_0^{+\infty} - \int_0^{+\infty} e^{-2v} dv \right) \\
&= -\frac{2}{\lambda} \left(0 + \int_0^{+\infty} -e^{-v} dv \right) + \frac{1}{\lambda} \left(0 + \frac{1}{2} \int_0^{+\infty} -2e^{-2v} dv \right) \\
&= -\frac{2}{\lambda} e^{-v} \Big|_0^{+\infty} + \frac{1}{2\lambda} e^{-2v} \Big|_0^{+\infty} \\
&= -\frac{2}{\lambda} (0 - 1) + \frac{1}{2\lambda} (0 - 1) \\
&= \frac{2}{\lambda} - \frac{1}{2\lambda} = \frac{3}{2\lambda}
\end{aligned}$$

Therefore, $E[\max(X, Y)] = \frac{3}{2\lambda}$